Foundation/FirstOrder/Arithmetic/Definability/Definable.lean
@@ -412,14 +412,14 @@ lemma imp (h₁ : Γ.alt-[m].Definable P) (h₂ : Γ-[m].Definable Q) :
     have e₁ := h₁.iff (v := v)
     have e₂ := h₂.iff (v := v)
     simp [Semiformula.negPi, imp_iff_not_or]
-    grind
+    tauto
   | 𝚷 =>
     rcases h₁ with ⟨p₁, h₁⟩; rcases h₂ with ⟨p₂, h₂⟩
     refine ⟨p₁.negSigma ⋎ p₂, fun v ↦ ?_⟩
     have e₁ := h₁.iff (v := v)
     have e₂ := h₂.iff (v := v)
     simp [Semiformula.negSigma, imp_iff_not_or]
-    grind
+    tauto
   | 𝚫 => exact impDelta h₁ h₂
 
 lemma biconditional (h₁ : 𝚫-[m].Definable P) (h₂ : 𝚫-[m].Definable Q) {Γ} :
