Foundation/Modal/Kripke/Logic/S4Point2.lean
@@ -103,7 +103,7 @@ instance : Modal.S4 ⪱ Modal.S4Point2 := by
       constructor;
       . simp only [Set.mem_setOf_eq]; refine { refl := by omega, trans := by omega; };
       . suffices ∃ x, (0 : M.World) ≺ x ∧ (∀ y, x ≺ y → y = 1) ∧ ∃ x, (0 : M.World) ≺ x ∧ ¬x ≺ 1 by
-          simpa [M, Semantics.Models, Satisfies];
+          simp [M, Semantics.Models, Satisfies]; tauto;
         use 1;
         refine ⟨by omega, ?_, ?_⟩;
         . intro y;
