Foundation/Modal/Neighborhood/Logic/EMCN4.lean
@@ -46,7 +46,7 @@ instance Neighborhood.finite_complete : Complete Modal.EMCN4 FrameClass.finite_E
   replace F_trans := Set.mem_setOf_eq.mp F_trans;
 
   let M : Model := ⟨F, V⟩;
-  apply quasiFilteringTransitiveFiltration M (Finset.toSet $ φ.subformulas ∪ (□⊤ : Formula ℕ).subformulas) (by simp) |>.filtration_satisfies _ (by grind) |>.mp;
+  apply quasiFilteringTransitiveFiltration M (↑(φ.subformulas ∪ (□⊤ : Formula ℕ).subformulas) : Set _) (by simp) |>.filtration_satisfies _ (by grind) |>.mp;
   apply hφ;
   apply Set.mem_setOf_eq.mpr;
   exact {
